# Problem

The sum of the squares of the first ten natural numbers is, 1^2 + 2^2 +...+ 10^2 = 385.

The square of the sum of the first ten natural numbers is, (1 + 2 +...+ 10)^2 = 55^2 = 3025.

Hence the difference between the sum of squares of the first ten natural numbers and the square of the sum is 3025 - 385 = 2640.

Find the difference between the sum of the squares of the first one hundred natural numbers and the square of the sum.

# Solution

**Trivial**

Looping over every natural number for both operations, then computing the difference.

*Note: The following two solutions are unnecessarily overdone for the fact that the trivial solution is already fairly quick.
I saw an opportunity to use a clever solution and dove headfirst into the approach.*

**Two Functions (Attempt 1)**

Both the sum of squares and the square of the sum can be turned into equations in terms of the last value.

The square of the sum is relatively trivial.  The sum of natural numbers up to x is `x (x + 1) / 2`, so we can just square that.

The sum of squares is a bit less trivial.  Looking at the differences between adjacent terms reveals that it follows a pattern indicating it is a cubic formula.

| x | Sum | f(x) = Sum(x) - Sum(x - 1) | g(x) = f(x) - f(x - 1) | h(x) = g(x) - g(x - 1) |
| - | --- | -------------------------- | ---------------------- | ---------------------- |
| 1 | 1   | 1                          | 1                      | 2                      |
| 2 | 5   | 4                          | 3                      | 2                      |
| 3 | 14  | 9                          | 5                      | 2                      |
| 4 | 30  | 16                         | 7                      | 2                      |
| 5 | 55  | 25                         | 9                      | 2                      |

4 points is sufficient to determine the cubic formula for the sum of squares.

```
----[d]----
Sum(x) = ax^3 + bx^2 + cx + d

d = -ax^3 - bx^2 - cx + Sum(x)

d = -a * 1^3 - b * 1^2 - c * 1 + 1
d = -a - b - c + 1

----[c]----

Sum(x) = ax^3 + bx^2 + cx + (-a - b - c + 1)
Sum(x) = a(x^3 - 1) + b(x^2 - 1) + c(x - 1) + 1

c(x - 1) = -a(x^3 - 1) - b(x^2 - 1) - 1 + Sum(x)
c = (-a(x^3 - 1) - b(x^2 - 1) - 1 + Sum(x)) / (x - 1)

c = (-a(2^3 - 1) - b(2^2 - 1) - 1 + 5) / (2 - 1)
c = (-a * 7 - b * 3 + 4) / 1
c = -7a - 3b + 4

----[b]----

Sum(x) = a(x^3 - 1) + b(x^2 - 1) + (-7a - 3b + 4)(x - 1) + 1
Sum(x) = a(x^3 - 1) + b(x^2 - 1) - 7ax + 7a - 3bx + 3b + 4x - 4 + 1
Sum(x) = a(x^3 - 1) + b(x^2 - 1) + a(-7x + 7) + b(-3x + 3) + 4x - 3
Sum(x) = a(x^3 - 1 - 7x + 7) + b(x^2 - 1 - 3x + 3) + 4x - 3
Sum(x) = a(x^3 - 7x + 6) + b(x^2 - 3x + 2) + 4x - 3

b(x^2 - 3x + 2) = -a(x^3 - 7x + 6) - 4x + 3 + Sum(x)
b = (-a(x^3 - 7x + 6) - 4x + 3 + Sum(x)) / (x^2 - 3x + 2)

b = (-a(3^3 - 7*3 + 6) - 4*3 + 3 + 14) / (3^2 - 3*3 + 2)
b = (-12a + 5) / 2
b = -6a + 5/2

----[a]----
Sum(x) = a(x^3 - 7x + 6) + (-6a + 5/2)(x^2 - 3x + 2) + 4x - 3
Sum(x) = ax^3 - 7ax + 6a + (-6ax^2 + 18ax - 12a + 5x^2/2 - 15x/2 + 5) + 4x - 3
Sum(x) = ax^3 - 6ax^2 + 11ax - 6a + 5x^2/2 - 7x/2 + 2
Sum(x) = a(x^3 - 6x^2 + 11x - 6) + (5x^2 - 7x + 4) / 2

a(x^3 - 6x^2 + 11x - 6) = -(5x^2 - 7x + 4) / 2 + Sum(x)
a = (-(5x^2 - 7x + 4) / 2 + Sum(x)) / (x^3 - 6x^2 + 11x - 6)

a = (-(5*4^2 - 7*4 + 4) / 2 + 30) / (4^3 - 6*4^2 + 11*4 - 6)
a = (-(80 - 28 + 4) / 2 + 30) / (64 - 96 + 44 - 6)
a = (-56 / 2 + 30) / 6
a = (-28 + 30) / 6
a = 2/6
a = 1/3

----[b]----
b = -6a + 5/2
b = -6 * 1/3 + 5/2
b = -2 + 5/2
b = (5 - 4) / 2
b = 1/2

----[c]----
c = -7a - 3b + 4
c = -7/3 - 3/2 + 4
c = (-14 - 9 + 24) / 6
c = 1/6

----[d]----
d = -a - b - c + 1
d = -1/3 - 1/2 - 1/6 + 1
d = (-2 - 3 - 1 + 6) / 6
d = 0/6

Sum(x) = x^3/3 + x^2/2 + x/6
```

Wow that was a fair amount of algebra, but it means we can calculate the sum of squares in just a handful of multiplications

**One Function (Attempt 2)**

Instead of having two separate polynomials we subtract, why not combine them into a single polynomial?

```
(x(x + 1) / 2)^2 - (x^3/3 + x^2/2 + x/6)
((x^2 + x) / 2)^2 - x^3/3 - x^2/2 - x/6

(x^4 + 2x^3 + x^2) / 4 - x^3/3 - x^2/2 - x/6
(6x^4 + 12x^3 + 6x^2 - 8x^3 - 12x^2 - 4x) / 24
(6x^4 + 4x^3 -6x^2 - 4x) / 24
(6x + 4)(x^3 - x) / 24
(3x + 2)(x^3 - x) / 12
```

Not nearly as much algebra, but we did build off the prior work.
This final expression allows us to compute the full result with only a single, relatively simple polynomial.